coq/Antimirov.v
@@ -1,21 +1,14 @@
-Require Import Regex.
+Require Import Regex ReCountable.
 
 (* If r is a regex and a is a char, then a partial derivative
    is a regex r' such that if r' accepts word s, then r accepts a ⋅ s.
    We can construct sets of partial derivatives (Antimirov derivatives). *)
-Print gset_empty.
-Print EqDecision.
-Print RelDecision.
-Print Countable.
 
-Parameter re_decidable : EqDecision re.
-Parameter re_countable : @Countable re re_decidable.
-
-Fixpoint a_der (r : re) (a : char) : gset re :=
+Fixpoint a_der (r : re) (a : char) `{Countable re} : gset re :=
   match r with
-  | Empty => @gset_empty re re_decidable re_countable
+  | Empty => gset_empty
   | Epsilon => gset_empty
-  | Atom b => if eq_dec a b then gset_singleton Epsilon else gset_empty
+  | Atom b => if char_dec a b then gset_singleton Epsilon else gset_empty
   | Union r1 r2 => gset_union (a_der r1 a) (a_der r2 a)
   | Concat r1 r2 => 
     if eps r1 
@@ -23,3 +16,4 @@ Fixpoint a_der (r : re) (a : char) : gset re :=
     else (set_map (fun r => Concat r r2) (a_der r1 a))
   | Star r => set_map (fun r' => Concat r' (Star r)) (a_der r a)
   end.
+  
