coq/ReCountable.v
@@ -1,0 +1,67 @@
+Require Import Regex.
+
+(* In order to use sets, we need to prove that regexes have 
+   decidable equality and are countable *)
+
+(* Injection from re to nat *)
+Definition encode_pair_pos (p : positive * positive) : positive := encode p.
+Definition encode_ascii (p : ascii) : positive := encode p.
+Definition decode_pair_pos (p : positive) : option (positive * positive) := decode p.
+Definition decode_ascii (p : positive) : option ascii := decode p.
+
+Fixpoint encode_regex (r : re) : positive :=
+  match r with
+  | Empty => encode_pair_pos (1%positive, 1%positive)
+  | Epsilon => encode_pair_pos (2%positive, 2%positive)
+  | Atom a => encode_pair_pos (3%positive, encode_ascii a)
+  | Union r1 r2 => encode_pair_pos
+    (4%positive, (encode_pair_pos (encode_regex r1, encode_regex r2)))
+  | Concat r1 r2 => encode_pair_pos 
+    (5%positive, (encode_pair_pos (encode_regex r1, encode_regex r2)))
+  | Star r' => encode_pair_pos (6%positive, (encode_regex r'))
+  end.
+
+Definition decode_regex (n : positive) : option re := 
+  match (decode_pair_pos n) with
+  | Some (1%positive, 1%positive) => Some Empty
+  | Some (2%positive, 2%positive) => Some Epsilon
+  | Some (3%positive, rest) =>
+    match (decode_ascii rest) with
+    | Some a => Some (Atom a)
+    | None => None
+    end
+    (* | Some (4, rest) =>
+      let (enc_r1, enc_r2) := decode rest in
+      match decode_regex enc_r1, decode_regex enc_r2 with
+      | Some r1, Some r2 => Some (Union r1 r2)
+      | _, _ => None
+      end
+    | Some (5, rest) =>
+      let (enc_r1, enc_r2) := decode rest in
+      match decode_regex enc_r1, decode_regex enc_r2 with
+      | Some r1, Some r2 => Some (Concat r1 r2)
+      | _, _ => None
+      end
+    | Some (6, rest) =>
+      match decode_regex rest with
+      | Some r => Some (Star r)
+      | None => None
+      end *)
+    | _ => None
+  end.
+
+Definition decode_encode_regex (r : re) : 
+  decode_regex (encode_regex r) = Some r.
+Proof. 
+  unfold decode_regex, encode_regex. induction r; 
+  unfold encode_pair_pos, decode_pair_pos, encode_ascii, decode_ascii;
+  rewrite ! decode_encode; eauto.
+  - 
+Admitted.
+
+
+Instance re_countable : @Countable re re_dec := {
+  encode := encode_regex;
+  decode := decode_regex;
+  decode_encode := decode_encode_regex
+}.
